theories/OrderedMonad.v
@@ -1,0 +1,133 @@
+Require Import Coq.Setoids.Setoid.
+Require Export PredMonad.OrderedType.
+
+Import ProperTermNotations.
+
+
+(***
+ *** The Monad Typeclass
+ ***)
+
+Class MonadOps (M : OrderedType -> OrderedType) : Type :=
+  { returnM : forall {A : OrderedType}, ProperTerm (A -o> M A);
+    bindM : forall {A B : OrderedType}, ProperTerm (M A -o> (A -o> M B) -o> M B) }.
+
+Class Monad M {MonadOps:MonadOps M} : Prop :=
+  {
+    monad_return_bind :
+      forall A B x (f: ProperTerm (A -o> M B)),
+        bindM @ (returnM @ x) @ f =o= f @ x;
+    monad_bind_return :
+      forall A (m:M A),
+        bindM @ m @ returnM =o= m;
+    monad_assoc :
+      forall A B C m (f:A -o> M B) (g:B -o> M C),
+        bindM @ (bindM @ m @ f) @ g
+        =o= bindM @ m @ (pfun (x ::: _) ==> !bindM @ (!f @ pvar x) @ !g)
+  }.
+
+
+(***
+ *** The Identity Monad
+ ***)
+
+Definition Identity (A: OrderedType) : OrderedType := A.
+Instance MonadOps_Identity : MonadOps Identity :=
+  { returnM := fun A => (pfun (x ::: A) ==> pvar x)%pterm;
+    bindM := fun A B =>
+               (pfun (m:::A) ==> pfun (f:::A -o> B) ==>
+                     pvar f @ pvar m)%pterm }.
+
+Instance Monad_Identity : Monad Identity.
+  constructor; intros.
+  destruct x as [x1 x2 pf_x]; destruct f as [f1 f2 pf_f]; compute.
+  destruct pf_f as [ pf_f1 pf_f2 pf_f3 ].
+  destruct pf_x as [ pf_x1 pf_x2 pf_x3 ].
+  split.
+  apply pf_f1; repeat constructor; apply pf_x1; repeat constructor.
+  apply pf_f1; repeat constructor; apply pf_x1; repeat constructor.
+  destruct m as [m1 m2 pf_m].
+  destruct pf_m as [ pf_m1 pf_m2 pf_m3 ].
+  compute; split; apply pf_m1; repeat constructor.
+  destruct m as [m1 m2 pf_m];
+    destruct pf_m as [ pf_m1 pf_m2 pf_m3 ].
+  destruct f as [f1 f2 pf_f];
+    destruct pf_f as [ pf_f1 pf_f2 pf_f3 ].
+  destruct g as [g1 g2 pf_g];
+    destruct pf_g as [ pf_g1 pf_g2 pf_g3 ].
+  compute; split; apply pf_g1; repeat constructor;
+    apply pf_f1; repeat constructor; apply pf_m1; repeat constructor.
+Qed.
+
+
+(***
+ *** The Set Monad
+ ***)
+
+(* The downward-closed sets, as an OrderedType *)
+Definition SetM (A: OrderedType) : OrderedType := ~o~ A -o> OTProp.
+
+(* Mapping the elements of a downward-closed set; this is the functor map
+operation for SetM *)
+Program Definition SetM_map {ctx} {A} {B}
+        (f: OTPairInCtx ctx (A -o> B))
+        (s: OTPairInCtx ctx (SetM A)) : OTPairInCtx ctx (SetM B) :=
+  pfun (y ::: ~o~ B) ==>
+       map3_OTPairInCtx
+         (ctx:= ~o~ B::ctx)
+         (A:= A -o> B) (B:=SetM A) (C:=~o~ B) (D:=OTProp)
+         (fun f s y =>
+            exists x, ot_R A x x /\ s x /\ ot_R B y (f x))
+         _ (!f) (!s) (pvar y).
+Next Obligation.
+  unfold Basics.impl.
+  intros f1 f2 pf_f s1 s2 pf_s y1 y2 pf_y.
+  destruct pf_f as [ pf_f1 pf_f2 pf_f3 ].
+  destruct pf_s as [ pf_s1 pf_s2 pf_s3 ].
+  destruct pf_y as [ pf_y1 pf_y2 pf_y3 ].
+  split; intro; try assumption.
+  repeat (destruct H); destruct H0.
+  exists x; repeat split.
+  assumption.
+  apply (pf_s3 x); try assumption.
+  split; assumption.
+  apply (semitransitivity (SemiTransitive:=B) _ y1); try assumption.
+  apply pf_f2; split; assumption.
+  apply (semitransitivity (SemiTransitive:=B) _ (f1 x)); try assumption.
+  apply pf_f1; split; assumption.
+  apply pf_f2; split; assumption.
+  apply pf_f3; split; assumption.
+Qed.
+
+(* Take the union of a set of sets; this is the join operation for SetM *)
+Program Definition SetM_union {ctx} {A}
+        (s: OTPairInCtx ctx (SetM (SetM A))) : OTPairInCtx ctx (SetM A) :=
+  pfun (x ::: ~o~ A) ==>
+       map2_OTPairInCtx (A:=SetM (SetM A)) (B:=~o~ A) (C:=OTProp)
+       (fun s x => exists s', ot_R (SetM A) s' s' /\ s s' /\ s' x) _ (!s) (pvar x).
+Next Obligation.
+  intros s1 s2 pf_s x1 x2 pf_x.
+  destruct pf_s as [ pf_s1 pf_s2 pf_s3 ].
+  destruct pf_x as [ pf_x1 pf_x2 pf_x3 ].
+  split; intro; try assumption.
+  destruct H as [ s' H ]; destruct H; destruct H0.
+  exists s'; repeat split.
+  apply H.
+  unfold Basics.impl in pf_s3; apply (pf_s3 s'); try assumption.
+  split; apply H; assumption.
+  unfold Basics.impl in H; apply (H x1).
+  split; assumption.
+  assumption.
+Qed.
+
+Instance MonadOps_SetM : MonadOps SetM :=
+  { returnM := fun A => (pfun (x ::: A) ==>
+                         pfun (y ::: ~o~ A) ==>
+                         proper_leq (pvar y) (pvar x))%pterm;
+    bindM := fun A B =>
+               (pfun (m:::SetM A) ==> pfun (f::: A -o> SetM B) ==>
+                  SetM_union (SetM_map (pvar f) (pvar m)))%pterm }.
+
+(*
+Instance Monad_SetM : Monad SetM.
+*)
